Port the malloc macros to the new proof style

theories/examples/macros_new.v
@@ -1,13 +1,13 @@
 From iris.algebra Require Import frac.
 From iris.proofmode Require Import tactics spec_patterns coq_tactics ltac_tactics reduction.
 Require Import Eqdep_dec List.
-From cap_machine Require Import classes rules (* logrel *) macros_helpers.
-From cap_machine Require Export iris_extra addr_reg_sample contiguous (* malloc *).
+From cap_machine Require Import classes rules logrel macros_helpers.
+From cap_machine Require Export iris_extra addr_reg_sample contiguous malloc.
 From cap_machine Require Import solve_pure proofmode.
 
 Section macros.
   Context {Σ:gFunctors} {memg:memG Σ} {regg:regG Σ}
-          (* {nainv: logrel_na_invs Σ} *)
+          {nainv: logrel_na_invs Σ}
           `{MP: MachineParameters}.
 
   (* --------------------------------------------------------------------------------- *)
@@ -57,7 +57,7 @@ Section macros.
     iDestruct (codefrag_contiguous_region with "Hprog") as %Hregion. (* TODO: automate this *)
     iGo "Hprog". instantiate (1 := pc_b). solve_addr.
     iGo "Hprog". iApply "Hφ"; iFrame.
-  Qed.
+ Qed.
 
   (* --------------------------------------------------------------------------------- *)
   (* ------------------------------------- ASSERT ------------------------------------ *)
@@ -123,7 +123,7 @@ Section macros.
             "(>Hprog & >HPC & >Hpc_b & >Ha_entry & >Hr & >Hr_t1 & >Hr_t2 & >Hr_t3 & Hφ)".
     subst w_r. rewrite {1}/assert_r_z_instrs.
     focus_block_0 "Hprog" as "Hfetch" "Hcont".
-    iApply (fetch_spec with "[-]"); iFrameCapSolve.
+    iApply fetch_spec; iFrameCapSolve.
     iNext. iIntros "(HPC & Hfetch & Hr1 & Hr2 & Hr3 & Hpc_b & Ha_entry)".
     unfocus_block "Hfetch" "Hcont" as "Hprog".
 
@@ -138,346 +138,100 @@ Section macros.
   (* Spec for assertion failure *)
   (* When the assertion fails, the program jumps to the failure subroutine, sets the
      flag (which by convention is one address after subroutine) and Fails *)
-  Lemma assert_r_z_fail a f_a r z pc_p pc_b pc_e a_first a_last z_r
+  Lemma assert_r_z_fail f_a r z pc_p pc_b pc_e a_first z_r
         b_link e_link a_link a_entry
-        f_b f_e f_a_first f_a_last a' a_env (* fail subroutine *)
-        flag_p flag_b flag_e flag_a (* flag capability *) :
-    isCorrectPC_range pc_p pc_b pc_e a_first a_last →
-    contiguous_between a a_first a_last →
+        f_b f_e f_a_first a_env (* fail subroutine *)
+        flag_p flag_b flag_e flag_a (* flag capability *)
+        w1 w2 w3 wf :
+    ExecPCPerm pc_p →
+    SubBounds pc_b pc_e a_first (a_first ^+ length (assert_r_z_instrs f_a r z))%a →
     (* linking table assumptions *)
     withinBounds (RW, b_link, e_link, a_entry) = true →
     (a_link + f_a)%a = Some a_entry ->
     (* failure subroutine assumptions *)
-    isCorrectPC_range RX f_b f_e f_a_first f_a_last →
-    contiguous_between a' f_a_first f_a_last →
-    (f_a_first + (length a'))%a = Some a_env ->
+    SubBounds f_b f_e f_a_first (f_a_first ^+ length assert_fail_instrs)%a →
+    (f_a_first + (length assert_fail_instrs))%a = Some a_env ->
     withinBounds (RX,f_b,f_e,a_env) = true ->
     (* flag assumptions *)
-    withinBounds (flag_p,flag_b,flag_e,flag_a) = true ∧ writeAllowed flag_p = true ->
-    (* condition for assertion success *)
+    withinBounds (flag_p,flag_b,flag_e,flag_a) = true →
+    writeAllowed flag_p = true ->
+    (* condition for assertion failure *)
     (z_r ≠ z) ->
 
     (* the assert and assert failure subroutine programs *)
-    {{{ ▷ assert_r_z a f_a r z
-    ∗ ▷ assert_fail a'
+    {{{ ▷ codefrag a_first (assert_r_z_instrs f_a r z)
+    ∗ ▷ codefrag f_a_first assert_fail_instrs
     ∗ ▷ PC ↦ᵣ inr (pc_p,pc_b,pc_e,a_first)
     (* linking table and assertion flag *)
     ∗ ▷ pc_b ↦ₐ inr (RO,b_link,e_link,a_link) (* the linking table capability *)
     ∗ ▷ a_entry ↦ₐ inr (E,f_b,f_e,f_a_first) (* the capability to the failure subroutine *)
     ∗ ▷ a_env ↦ₐ inr (flag_p,flag_b,flag_e,flag_a) (* the assertion flag capability *)
-    ∗ ▷ (∃ w, flag_a ↦ₐ w) (* the assertion flag *)
+    ∗ ▷ flag_a ↦ₐ wf (* the assertion flag *)
     (* registers *)
     ∗ ▷ r ↦ᵣ inl z_r
-    ∗ ▷ (∃ w, r_t1 ↦ᵣ w)
-    ∗ ▷ (∃ w, r_t2 ↦ᵣ w)
-    ∗ ▷ (∃ w, r_t3 ↦ᵣ w) }}}
+    ∗ ▷ r_t1 ↦ᵣ w1
+    ∗ ▷ r_t2 ↦ᵣ w2
+    ∗ ▷ r_t3 ↦ᵣ w3 }}}
       
       Seq (Instr Executable)
       
     {{{ RET FailedV; r_t1 ↦ᵣ inl 0%Z ∗ r_t2 ↦ᵣ inl 0%Z ∗ r_t3 ↦ᵣ inl 0%Z ∗ (∃ z, r ↦ᵣ inl z ∧ ⌜z ≠ 0⌝)
-         ∗ PC ↦ᵣ inr (RX, f_b, f_e,^(f_a_last + (-1))%a)
-         ∗ assert_r_z a f_a r z ∗ assert_fail a'
+         ∗ PC ↦ᵣ inr (RX, f_b, f_e, (f_a_first ^+ (length assert_fail_instrs - 1))%a)
+         ∗ codefrag a_first (assert_r_z_instrs f_a r z)
+         ∗ codefrag f_a_first assert_fail_instrs
          ∗ pc_b ↦ₐ inr (RO,b_link,e_link,a_link) ∗ a_entry ↦ₐ inr (E,f_b,f_e,f_a_first)
          ∗ a_env ↦ₐ inr (flag_p,flag_b,flag_e,flag_a) ∗ flag_a ↦ₐ inl 1%Z }}}.
   Proof.
-    iIntros (Hvpc Hcont Hwb Htable Hvpc' Hcont' Henv Henvwb [Hwb' Hwa] Hfailure φ)
+    iIntros (Hexpc Hsub Hwb Htable Hsub' Henv Henvwb Hwb' Hwa Hfailure φ)
             "(>Hprog & >Hprog' & >HPC & >Hpc_b & >Ha_entry & >Ha_env & >Hflag & >Hr & >Hr_t1 & >Hr_t2 & >Hr_t3) Hφ".
-    iDestruct "Hflag" as (flag_w) "Hflag".
-    (* fetch f *)
-    iDestruct (contiguous_between_program_split with "Hprog") as (fetch_prog rest link)
-                                                                   "(Hfetch & Hprog & #Hcont)";[apply Hcont|].
-    iDestruct "Hcont" as %(Hcont_fetch & Hcont_rest & Heqapp & Hlink).
-    iDestruct "Hr_t1" as (w1) "Hr_t1".
-    iDestruct "Hr_t2" as (w2) "Hr_t2".
-    iDestruct "Hr_t3" as (w3) "Hr_t3".
-    iApply (fetch_spec with "[$HPC $Hfetch $Hr_t1 $Hr_t2 $Hr_t3 $Ha_entry $Hpc_b Hφ Hprog Hr Hprog' Ha_env Hflag]");
-      [|apply Hcont_fetch|apply Hwb|apply Htable|].
-    { intros mid Hmid. apply isCorrectPC_inrange with a_first a_last; auto.
-      apply contiguous_between_bounds in Hcont_rest. revert Hcont_rest Hmid; clear. solve_addr. }
-    iNext. iIntros "(HPC & Hfetch& Hr_t1 & Hr_t2 & Hr_t3 & Hpc_b & Ha_entry)".
-    iDestruct (big_sepL2_length with "Hprog") as %Hlength_rest.
-    assert (isCorrectPC_range pc_p pc_b pc_e link a_last) as Hvpc_rest.
-    { intros mid Hmid. apply isCorrectPC_inrange with a_first a_last; auto. revert Hmid Hlink;clear. solve_addr. }
-    destruct rest as [|a0 l'];[inversion Hlength_rest|].
-    apply contiguous_between_cons_inv_first in Hcont_rest as Heq. subst a0.
-    (* sub_r_z r r z *)
-    destruct l';[inversion Hlength_rest|].
-    iPrologue "Hprog".
-    iApply (wp_add_sub_lt_success_dst_z with "[$HPC $Hi $Hr]");
-      [apply decode_encode_instrW_inv|right;left;eauto|iContiguous_next Hcont_rest 0|iCorrectPC link a_last|..].
-    iEpilogue "(HPC & Hi & Hr)"; iCombine "Hi" "Hfetch" as "Hprog_done".
-    (* jnz r_t1 r *)
-    iPrologue "Hprog".
-    iApply (wp_jnz_success_jmp with "[$HPC $Hi $Hr_t1 $Hr]");
-      [apply decode_encode_instrW_inv|iCorrectPC link a_last|simpl;revert Hfailure;clear;intros Hne Hcontr;simplify_eq;lia|..].
-    iEpilogue "(HPC & Hi & Hr_t1 & Hr)"; iSimpl in "HPC"; iCombine "Hi" "Hprog_done" as "Hprog_done".
-    iCombine "Hprog" "Hprog_done" as "Hprog_done".
-    (* FAILURE SUBROUTINE *)
-    iDestruct (big_sepL2_length with "Hprog'") as %Hlength'.
-    destruct a';[inversion Hlength'|].
-    apply contiguous_between_cons_inv_first in Hcont' as Heq. subst a1.
-    (* move r_t1 PC *)
-    destruct a';[inversion Hlength'|].
-    iAssert (⌜r_t1 ≠ PC⌝)%I as %Hne.
-    { iIntros (Hcontr). rewrite Hcontr. iDestruct (regname_dupl_false with "Hr_t1 HPC") as "H". done. }
-    iPrologue "Hprog'".
-    iApply (wp_move_success_reg_fromPC with "[$HPC $Hi $Hr_t1]");
-      [apply decode_encode_instrW_inv|iCorrectPC f_a_first f_a_last|iContiguous_next Hcont' 0|auto|..].
-    iEpilogue "(HPC & Hi & Hr_t1)". iRename "Hi" into "Hprog_done'".
-    (* lea r_t1 5 *)
-    destruct a';[inversion Hlength'|].
-    iPrologue "Hprog".
-    assert ((f_a_first + 6)%a = Some a_env) as Hlea.
-    { simpl in Henv. inversion Hlength' as [Heq]. rewrite Heq in Henv. auto. }
-    iApply (wp_lea_success_z with "[$HPC $Hi $Hr_t1]");
-      [apply decode_encode_instrW_inv|iCorrectPC f_a_first f_a_last|iContiguous_next Hcont' 1|apply Hlea|auto..].
-    iEpilogue "(HPC & Hi & Hr_t1)". iCombine "Hi" "Hprog_done'" as "Hprog_done'".
-    (* load r_t1 r_t1 *)
-    destruct a';[inversion Hlength'|].
-    iPrologue "Hprog".
-    iAssert (⌜(a_env =? a2)%a = false⌝)%I as %Hne'.
-    { destruct (decide (a_env = a2)%Z); [subst|iPureIntro;apply Z.eqb_neq,neq_z_of;auto].
-      iDestruct (mapsto_valid_2 with "Hi Ha_env") as %?. done. }
-    iApply (wp_load_success_same with "[$HPC $Hi $Hr_t1 Ha_env]");
-      [|apply decode_encode_instrW_inv|iCorrectPC f_a_first f_a_last|split;auto|iContiguous_next Hcont' 2|
-       rewrite Hne';iFrame|rewrite Hne'];auto.
-    iEpilogue "(HPC & Hr_t1 & Hi & Ha_env)". iCombine "Hi" "Hprog_done" as "Hprog_done".
-    (* store r_t1 1 *)
-    destruct a';[inversion Hlength'|].
-    iPrologue "Hprog".
-    iApply (wp_store_success_z with "[$HPC $Hi $Hr_t1 $Hflag]");
-      [apply decode_encode_instrW_inv|iCorrectPC f_a_first f_a_last|iContiguous_next Hcont' 3|
-       split;auto|].
-    iEpilogue "(HPC & Hi & Hr_t1 & Hflag)"; iCombine "Hi" "Hprog_done" as "Hprog_done".
-    (* move r_t1 0 *)
-    destruct a';[inversion Hlength'|].
-    iPrologue "Hprog".
-    iApply (wp_move_success_z with "[$HPC $Hi $Hr_t1]");
-      [apply decode_encode_instrW_inv|iCorrectPC f_a_first f_a_last|iContiguous_next Hcont' 4|].
-    iEpilogue "(HPC & Hi & Hr_t1)"; iCombine "Hi" "Hprog_done" as "Hprog_done".
-    (* Halt *)
-    destruct a';[|inversion Hlength'].
-    apply contiguous_between_last with (ai:=a5) in Hcont' as Hlink';[|auto].
-    iPrologue "Hprog".
-    iApply (wp_fail with "[$HPC $Hi]");
-      [apply decode_encode_instrW_inv|iCorrectPC f_a_first f_a_last|].
-    iEpilogue "(HPC & Hi)".
-    iApply wp_value. iApply "Hφ".
-    iFrame. iSplitL "Hr".
-    { simpl. iExists _. iFrame. iPureIntro. revert Hfailure. clear. lia. }
-    assert ((f_a_last + (-1))%a = Some a5) as ->;[|simpl].
-    { eapply contiguous_between_last in Hcont';[|eauto]. revert Hlink' Hcont'. clear. solve_addr. }
-    iFrame. rewrite Heqapp. iDestruct "Hprog_done'" as "(?&?)". iDestruct "Hprog_done" as "(?&?&?&?&?&?&?)".
-    iFrame.
+    rewrite {1}/assert_r_z_instrs.
+    focus_block_0 "Hprog" as "Hfetch" "Hcont".
+    iApply fetch_spec; iFrameCapSolve.
+    iNext. iIntros "(HPC & Hfetch & Hr_t1 & Hr_t2 & Hr_t3 & Hpc_b & Ha_entry)".
+    unfocus_block "Hfetch" "Hcont" as "Hprog".
+
+    focus_block 1 "Hprog" as amid1 Hamid1 "Hprog" "Hcont".
+    iInstr "Hprog".
+    iInstr "Hprog". by intros HH; inversion HH; lia.
+    unfocus_block "Hprog" "Hcont" as "Hprog".
+
+    rewrite {1}/assert_fail_instrs.
+    codefrag_facts "Hprog'". iGo "Hprog'".
+    wp_end. iApply "Hφ". iFrame. iExists _. iFrame. iPureIntro. lia.
   Qed.
-    
+
   (* --------------------------------------------------------------------------------- *)
   (* ------------------------------------- MALLOC ------------------------------------ *)
   (* --------------------------------------------------------------------------------- *)
 
   (* malloc stores the result in r_t1, rather than a user chosen destination. 
      f_m is the offset of the malloc capability *)
-  Definition malloc_instrs f_m size :=
+  Definition malloc_instrs f_m (size: Z) :=
     fetch_instrs f_m ++
-    [move_r r_t5 r_t0;
-    move_r r_t3 r_t1;
-    move_z r_t1 size;
-    move_r r_t0 PC;
-    lea_z r_t0 3;
-    jmp r_t3;
-    move_r r_t0 r_t5;
-    move_z r_t5 0].
-
-  Definition malloc f_m size a : iProp Σ :=
-    ([∗ list] a_i;w_i ∈ a;(malloc_instrs f_m size), a_i ↦ₐ w_i)%I.
+    encodeInstrsW [
+     Mov r_t5 r_t0;
+     Mov r_t3 r_t1;
+     Mov r_t1 size;
+     Mov r_t0 PC;
+     Lea r_t0 3;
+     Jmp r_t3;
+     Mov r_t0 r_t5;
+     Mov r_t5 0
+  ].
 
   (* malloc spec *)
-  Lemma malloc_spec φ size cont a pc_p pc_b pc_e a_first a_last
+  Lemma malloc_spec_alt φ ψ size cont pc_p pc_b pc_e a_first
         b_link e_link a_link f_m a_entry mallocN b_m e_m EN rmap :
-    isCorrectPC_range pc_p pc_b pc_e a_first a_last →
-    contiguous_between a a_first a_last →
+    ExecPCPerm pc_p →
+    SubBounds pc_b pc_e a_first (a_first ^+ length (malloc_instrs f_m size))%a →
     withinBounds (RW, b_link, e_link, a_entry) = true →
     (a_link + f_m)%a = Some a_entry →
     dom (gset RegName) rmap = all_registers_s ∖ {[ PC; r_t0 ]} →
     ↑mallocN ⊆ EN →
-    size > 0 →
+    (size > 0)%Z →
 
     (* malloc program and subroutine *)
-    ▷ malloc f_m size a
-    ∗ na_inv logrel_nais mallocN (malloc_inv b_m e_m)
-    ∗ na_own logrel_nais EN
-    (* we need to assume that the malloc capability is in the linking table at offset f_m *)
-    ∗ ▷ pc_b ↦ₐ inr (RO,b_link,e_link,a_link)
-    ∗ ▷ a_entry ↦ₐ inr (E,b_m,e_m,b_m)
-    (* register state *)
-    ∗ ▷ PC ↦ᵣ inr (pc_p,pc_b,pc_e,a_first)
-    ∗ ▷ r_t0 ↦ᵣ cont
-    ∗ ▷ ([∗ map] r_i↦w_i ∈ rmap, r_i ↦ᵣ w_i)
-    (* continuation *)
-    ∗ ▷ (PC ↦ᵣ inr (pc_p,pc_b,pc_e,a_last) ∗ malloc f_m size a
-         ∗ pc_b ↦ₐ inr (RO,b_link,e_link,a_link)
-         ∗ a_entry ↦ₐ inr (E,b_m,e_m,b_m)
-         (* the newly allocated region *)
-         ∗ (∃ (b e : Addr),
-            ⌜(b + size)%a = Some e⌝
-            ∗ r_t1 ↦ᵣ inr (RWX,b,e,b)
-            ∗ [[b,e]] ↦ₐ [[region_addrs_zeroes b e]])
-         ∗ r_t0 ↦ᵣ cont
-         ∗ na_own logrel_nais EN
-         ∗ ([∗ map] r_i↦w_i ∈ (<[r_t2:=inl 0%Z]>
-                               (<[r_t3:=inl 0%Z]>
-                                (<[r_t4:=inl 0%Z]>
-                                 (<[r_t5:=inl 0%Z]> (delete r_t1 rmap))))), r_i ↦ᵣ w_i)
-         (* the newly allocated region is fresh in the current world *)
-         (* ∗ ⌜Forall (λ a, a ∉ dom (gset Addr) (std W)) (region_addrs b e)⌝ *)
-         -∗ WP Seq (Instr Executable) {{ φ }})
-    ⊢
-      WP Seq (Instr Executable) {{ λ v, φ v ∨ ⌜v = FailedV⌝ }}.
-  Proof.
-    iIntros (Hvpc Hcont Hwb Ha_entry Hrmap_dom HmallocN Hsize)
-            "(>Hprog & #Hmalloc & Hna & >Hpc_b & >Ha_entry & >HPC & >Hr_t0 & >Hregs & Hφ)".
-    (* extract necessary registers from regs *)
-    iDestruct (big_sepL2_length with "Hprog") as %Hlength.
-    assert (is_Some (rmap !! r_t1)) as [rv1 ?]. by rewrite elem_of_gmap_dom Hrmap_dom; set_solver.
-    iDestruct (big_sepM_delete _ _ r_t1 with "Hregs") as "[Hr_t1 Hregs]"; eauto.
-    assert (is_Some (rmap !! r_t2)) as [rv2 ?]. by rewrite elem_of_gmap_dom Hrmap_dom; set_solver.
-    iDestruct (big_sepM_delete _ _ r_t2 with "Hregs") as "[Hr_t2 Hregs]". by rewrite lookup_delete_ne //.
-    assert (is_Some (rmap !! r_t3)) as [rv3 ?]. by rewrite elem_of_gmap_dom Hrmap_dom; set_solver.
-    iDestruct (big_sepM_delete _ _ r_t3 with "Hregs") as "[Hr_t3 Hregs]". by rewrite !lookup_delete_ne //.
-    assert (is_Some (rmap !! r_t5)) as [rv5 ?]. by rewrite elem_of_gmap_dom Hrmap_dom; set_solver.
-    iDestruct (big_sepM_delete _ _ r_t5 with "Hregs") as "[Hr_t5 Hregs]". by rewrite !lookup_delete_ne //.
-    destruct a as [|a l];[inversion Hlength|].
-    apply contiguous_between_cons_inv_first in Hcont as Heq. subst.
-    (* fetch f *)
-    iDestruct (contiguous_between_program_split with "Hprog") as (fetch_prog rest link)
-                                                                   "(Hfetch & Hprog & #Hcont)";[apply Hcont|].
-    iDestruct "Hcont" as %(Hcont_fetch & Hcont_rest & Heqapp & Hlink).
-    iApply (fetch_spec with "[- $HPC $Hfetch $Hr_t1 $Hr_t2 $Hr_t3 $Ha_entry $Hpc_b]");
-      [|apply Hcont_fetch|apply Hwb|apply Ha_entry|].
-    { intros mid Hmid. apply isCorrectPC_inrange with a_first a_last; auto.
-      apply contiguous_between_bounds in Hcont_rest. revert Hcont_rest Hmid; clear. solve_addr. }
-    iNext. iIntros "(HPC & Hfetch& Hr_t1 & Hr_t2 & Hr_t3 & Hpc_b & Ha_entry)".
-    iDestruct (big_sepL2_length with "Hprog") as %Hlength_rest.
-    assert (isCorrectPC_range pc_p pc_b pc_e link a_last) as Hvpc_rest.
-    { intros mid Hmid. apply isCorrectPC_inrange with a_first a_last; auto. revert Hmid Hlink;clear. solve_addr. }
-    destruct rest as [|a l'];[inversion Hlength_rest|].
-    apply contiguous_between_cons_inv_first in Hcont_rest as Heq. subst.
-    (* move r_t5 r_t0 *)
-    destruct l';[inversion Hlength_rest|].
-    iPrologue "Hprog".
-    iApply (wp_move_success_reg with "[$HPC $Hi $Hr_t5 $Hr_t0]");
-      [apply decode_encode_instrW_inv|iCorrectPC link a_last|iContiguous_next Hcont_rest 0|auto|..].
-    iEpilogue "(HPC & Hprog_done & Hr_t5 & Hr_t0)". iCombine "Hprog_done" "Hfetch" as "Hprog_done".
-    (* move r_t3 r_t1 *)
-    destruct l';[inversion Hlength_rest|].
-    iPrologue "Hprog".
-    iApply (wp_move_success_reg with "[$HPC $Hi $Hr_t3 $Hr_t1]");
-      [apply decode_encode_instrW_inv|iCorrectPC link a_last|iContiguous_next Hcont_rest 1|auto|..].
-    iEpilogue "(HPC & Hi & Hr_t3 & Hr_t1)"; iCombine "Hi" "Hprog_done" as "Hprog_done".
-    (* move r_t1 size *)
-    destruct l';[inversion Hlength_rest|].
-    iPrologue "Hprog".
-    iApply (wp_move_success_z with "[$HPC $Hi $Hr_t1]");
-      [apply decode_encode_instrW_inv|iCorrectPC link a_last|iContiguous_next Hcont_rest 2|auto|..].
-    iEpilogue "(HPC & Hi & Hr_t1)"; iCombine "Hi" "Hprog_done" as "Hprog_done".
-    (* move r_t0 PC *)
-    destruct l';[inversion Hlength_rest|].
-    iPrologue "Hprog".
-    iApply (wp_move_success_reg_fromPC with "[$HPC $Hi $Hr_t0]");
-      [apply decode_encode_instrW_inv|iCorrectPC link a_last|iContiguous_next Hcont_rest 3|auto|..].
-    iEpilogue "(HPC & Hi & Hr_t0)"; iCombine "Hi" "Hprog_done" as "Hprog_done".
-    (* lea r_t0 3 *)
-    destruct l';[inversion Hlength_rest|]. destruct l';[inversion Hlength_rest|].
-    iPrologue "Hprog".
-    assert ((a1 + 3)%a = Some a4) as Hlea.
-    { apply (contiguous_between_incr_addr_middle _ _ _ 3 3 a1 a4) in Hcont_rest; auto. }
-    iApply (wp_lea_success_z with "[$HPC $Hi $Hr_t0]");
-      [apply decode_encode_instrW_inv|iCorrectPC link a_last|iContiguous_next Hcont_rest 4|apply Hlea|auto..].
-    { apply contiguous_between_length in Hcont.
-      apply isCorrectPC_range_perm in Hvpc; [|revert Hcont; clear; solve_addr].
-      destruct Hvpc as [-> | -> ]; auto. }
-    iEpilogue "(HPC & Hi & Hr_t0)"; iCombine "Hi" "Hprog_done" as "Hprog_done".
-    (* jmp r_t3 *)
-    destruct l';[inversion Hlength_rest|].
-    iPrologue "Hprog".
-    iApply (wp_jmp_success with "[$HPC $Hi $Hr_t3]");
-      [apply decode_encode_instrW_inv|iCorrectPC link a_last|].
-    iEpilogue "(HPC & Hi & Hr_t3) /="; iCombine "Hi" "Hprog_done" as "Hprog_done".
-    (* we are now ready to use the malloc subroutine spec. For this we prepare the registers *)
-    iDestruct (big_sepM_insert _ _ r_t3 with "[$Hregs $Hr_t3]") as "Hregs".
-      by rewrite lookup_delete_ne // lookup_delete.
-    iDestruct (big_sepM_insert _ _ r_t2 with "[$Hregs $Hr_t2]") as "Hregs".
-      by rewrite lookup_insert_ne // lookup_delete_ne // lookup_delete_ne // lookup_delete.
-    rewrite -(delete_insert_ne _ r_t5 r_t3) // insert_delete.
-    rewrite -(delete_insert_ne _ r_t5 r_t2) // (insert_commute _ r_t2 r_t3) //.
-    rewrite insert_delete.
-    iDestruct (big_sepM_insert _ _ r_t5 with "[$Hregs $Hr_t5]") as "Hregs".
-      by rewrite lookup_delete. rewrite insert_delete.
-    iApply (wp_wand with "[-]").
-    iApply (simple_malloc_subroutine_spec with "[- $Hmalloc $Hna $Hregs $Hr_t0 $HPC $Hr_t1]"); auto.
-    { rewrite !dom_insert_L dom_delete_L Hrmap_dom.
-      rewrite !difference_difference_L !singleton_union_difference_L !all_registers_union_l.
-      f_equal. set_solver-. }
-    (* { lia. } *)
-    iNext.
-    rewrite updatePcPerm_cap_non_E.
-    2: { eapply isCorrectPC_range_perm_non_E; eauto.
-         generalize (contiguous_between_length _ _ _ Hcont_rest). cbn.
-         clear; solve_addr. }
-    iIntros "((Hna & Hregs) & Hr_t0 & HPC & Hbe) /=".
-    iDestruct "Hbe" as (b e size' Hsize' Hbe) "(Hr_t1 & Hbe)". inversion Hsize'; subst size'.
-    iDestruct (big_sepM_delete _ _ r_t3 with "Hregs") as "[Hr_t3 Hregs]".
-      by rewrite lookup_insert_ne // lookup_insert //.
-      rewrite delete_insert_ne // delete_insert_delete.
-      repeat (rewrite delete_insert_ne //;[]). rewrite delete_insert_delete.
-    iDestruct (big_sepM_delete _ _ r_t5 with "Hregs") as "[Hr_t5 Hregs]".
-      by (repeat (rewrite lookup_insert_ne //;[]); rewrite lookup_insert //).
-      repeat (rewrite delete_insert_ne //;[]). rewrite delete_insert_delete.
-    (* move r_t0 r_t5 *)
-    iPrologue "Hprog".
-    iApply (wp_move_success_reg with "[$HPC $Hi $Hr_t0 $Hr_t5]");
-      [apply decode_encode_instrW_inv|iCorrectPC link a_last|iContiguous_next Hcont_rest 6|auto|..].
-    iEpilogue "(HPC & Hi & Hr_t0 & Hr_t5)"; iCombine "Hi" "Hprog_done" as "Hprog_done".
-    (* move r_t5 0 *)
-    destruct l';[| by inversion Hlength_rest].
-    iPrologue "Hprog".
-    apply contiguous_between_last with (ai:=a5) in Hcont_rest as Hlast;[|auto].
-    iApply (wp_move_success_z with "[$HPC $Hi $Hr_t5]");
-      [apply decode_encode_instrW_inv|iCorrectPC link a_last|apply Hlast|auto|..].
-    iEpilogue "(HPC & Hi & Hr_t5)"; iCombine "Hi" "Hprog_done" as "Hprog_done".
-    (* continuation *)
-    iApply "Hφ".
-    iFrame "HPC". iSplitL "Hprog_done".
-    { rewrite Heqapp. repeat (iDestruct "Hprog_done" as "[$ Hprog_done]"). iFrame. done. }
-    iFrame.
-    iDestruct (big_sepM_insert _ _ r_t5 with "[$Hregs $Hr_t5]") as "Hregs".
-      repeat (rewrite lookup_insert_ne //;[]). apply lookup_delete.
-    iDestruct (big_sepM_insert _ _ r_t3 with "[$Hregs $Hr_t3]") as "Hregs".
-      repeat (rewrite lookup_insert_ne //;[]).
-      rewrite lookup_delete_ne // lookup_delete //.
-    repeat (rewrite (insert_commute _ r_t5) //;[]).
-    rewrite insert_delete -(delete_insert_ne _ _ r_t5) //.
-    rewrite (insert_commute _ r_t5 r_t2) // (delete_insert_ne _ r_t3 r_t2)//.
-    rewrite (insert_commute _ r_t4 r_t2) // insert_insert.
-    rewrite (insert_commute _ r_t3 r_t2) //.
-    rewrite -(delete_insert_ne _ r_t3) // insert_delete.
-    iFrame.
-    iExists b,e. iFrame. auto. auto.
-  Qed.
-
-  (* malloc spec - alternative formulation *)
-  Lemma malloc_spec_alt φ ψ size cont a pc_p pc_b pc_e a_first a_last
-        b_link e_link a_link f_m a_entry mallocN b_m e_m EN rmap :
-    isCorrectPC_range pc_p pc_b pc_e a_first a_last →
-    contiguous_between a a_first a_last →
-    withinBounds (RW, b_link, e_link, a_entry) = true →
-    (a_link + f_m)%a = Some a_entry →
-    dom (gset RegName) rmap = all_registers_s ∖ {[ PC; r_t0 ]} →
-    ↑mallocN ⊆ EN →
-    size > 0 →
-
-    (* malloc program and subroutine *)
-    ▷ malloc f_m size a
+    ▷ codefrag a_first (malloc_instrs f_m size)
     ∗ na_inv logrel_nais mallocN (malloc_inv b_m e_m)
     ∗ na_own logrel_nais EN
     (* we need to assume that the malloc capability is in the linking table at offset f_m *)
@@ -489,8 +243,9 @@ Section macros.
     ∗ ▷ ([∗ map] r_i↦w_i ∈ rmap, r_i ↦ᵣ w_i)
     (* failure/continuation *)
     ∗ ▷ (∀ v, ψ v -∗ φ v)
-    ∗ ▷ (ψ FailedV)
-    ∗ ▷ (PC ↦ᵣ inr (pc_p,pc_b,pc_e,a_last) ∗ malloc f_m size a
+    ∗ ▷ (φ FailedV)
+    ∗ ▷ (PC ↦ᵣ inr (pc_p,pc_b,pc_e,(a_first ^+ length (malloc_instrs f_m size))%a)
+         ∗ codefrag a_first (malloc_instrs f_m size)
          ∗ pc_b ↦ₐ inr (RO,b_link,e_link,a_link)
          ∗ a_entry ↦ₐ inr (E,b_m,e_m,b_m)
          (* the newly allocated region *)
@@ -522,63 +277,15 @@ Section macros.
     iDestruct (big_sepM_delete _ _ r_t3 with "Hregs") as "[Hr_t3 Hregs]". by rewrite !lookup_delete_ne //.
     assert (is_Some (rmap !! r_t5)) as [rv5 ?]. by rewrite elem_of_gmap_dom Hrmap_dom; set_solver.
     iDestruct (big_sepM_delete _ _ r_t5 with "Hregs") as "[Hr_t5 Hregs]". by rewrite !lookup_delete_ne //.
-    destruct a as [|a l];[inversion Hlength|].
-    apply contiguous_between_cons_inv_first in Hcont as Heq. subst.
-    (* fetch f *)
-    iDestruct (contiguous_between_program_split with "Hprog") as (fetch_prog rest link)
-                                                                   "(Hfetch & Hprog & #Hcont)";[apply Hcont|].
-    iDestruct "Hcont" as %(Hcont_fetch & Hcont_rest & Heqapp & Hlink).
-    iApply (fetch_spec with "[- $HPC $Hfetch $Hr_t1 $Hr_t2 $Hr_t3 $Ha_entry $Hpc_b]");
-      [|apply Hcont_fetch|apply Hwb|apply Ha_entry|].
-    { intros mid Hmid. apply isCorrectPC_inrange with a_first a_last; auto.
-      apply contiguous_between_bounds in Hcont_rest. revert Hcont_rest Hmid; clear. solve_addr. }
-    iNext. iIntros "(HPC & Hfetch& Hr_t1 & Hr_t2 & Hr_t3 & Hpc_b & Ha_entry)".
-    iDestruct (big_sepL2_length with "Hprog") as %Hlength_rest.
-    assert (isCorrectPC_range pc_p pc_b pc_e link a_last) as Hvpc_rest.
-    { intros mid Hmid. apply isCorrectPC_inrange with a_first a_last; auto. revert Hmid Hlink;clear. solve_addr. }
-    destruct rest as [|a l'];[inversion Hlength_rest|].
-    apply contiguous_between_cons_inv_first in Hcont_rest as Heq. subst.
-    (* move r_t5 r_t0 *)
-    destruct l';[inversion Hlength_rest|].
-    iPrologue "Hprog".
-    iApply (wp_move_success_reg with "[$HPC $Hi $Hr_t5 $Hr_t0]");
-      [apply decode_encode_instrW_inv|iCorrectPC link a_last|iContiguous_next Hcont_rest 0|auto|..].
-    iEpilogue "(HPC & Hprog_done & Hr_t5 & Hr_t0)". iCombine "Hprog_done" "Hfetch" as "Hprog_done".
-    (* move r_t3 r_t1 *)
-    destruct l';[inversion Hlength_rest|].
-    iPrologue "Hprog".
-    iApply (wp_move_success_reg with "[$HPC $Hi $Hr_t3 $Hr_t1]");
-      [apply decode_encode_instrW_inv|iCorrectPC link a_last|iContiguous_next Hcont_rest 1|auto|..].
-    iEpilogue "(HPC & Hi & Hr_t3 & Hr_t1)"; iCombine "Hi" "Hprog_done" as "Hprog_done".
-    (* move r_t1 size *)
-    destruct l';[inversion Hlength_rest|].
-    iPrologue "Hprog".
-    iApply (wp_move_success_z with "[$HPC $Hi $Hr_t1]");
-      [apply decode_encode_instrW_inv|iCorrectPC link a_last|iContiguous_next Hcont_rest 2|auto|..].
-    iEpilogue "(HPC & Hi & Hr_t1)"; iCombine "Hi" "Hprog_done" as "Hprog_done".
-    (* move r_t0 PC *)
-    destruct l';[inversion Hlength_rest|].
-    iPrologue "Hprog".
-    iApply (wp_move_success_reg_fromPC with "[$HPC $Hi $Hr_t0]");
-      [apply decode_encode_instrW_inv|iCorrectPC link a_last|iContiguous_next Hcont_rest 3|auto|..].
-    iEpilogue "(HPC & Hi & Hr_t0)"; iCombine "Hi" "Hprog_done" as "Hprog_done".
-    (* lea r_t0 3 *)
-    destruct l';[inversion Hlength_rest|]. destruct l';[inversion Hlength_rest|].
-    iPrologue "Hprog".
-    assert ((a1 + 3)%a = Some a4) as Hlea.
-    { apply (contiguous_between_incr_addr_middle _ _ _ 3 3 a1 a4) in Hcont_rest; auto. }
-    iApply (wp_lea_success_z with "[$HPC $Hi $Hr_t0]");
-      [apply decode_encode_instrW_inv|iCorrectPC link a_last|iContiguous_next Hcont_rest 4|apply Hlea|auto..].
-    { apply contiguous_between_length in Hcont.
-      apply isCorrectPC_range_perm in Hvpc; [|revert Hcont; clear; solve_addr].
-      destruct Hvpc as [-> | -> ]; auto. }
-    iEpilogue "(HPC & Hi & Hr_t0)"; iCombine "Hi" "Hprog_done" as "Hprog_done".
-    (* jmp r_t3 *)
-    destruct l';[inversion Hlength_rest|].
-    iPrologue "Hprog".
-    iApply (wp_jmp_success with "[$HPC $Hi $Hr_t3]");
-      [apply decode_encode_instrW_inv|iCorrectPC link a_last|].
-    iEpilogue "(HPC & Hi & Hr_t3) /="; iCombine "Hi" "Hprog_done" as "Hprog_done".
+
+    rewrite {1}/malloc_instrs.
+    focus_block_0 "Hprog" as "Hfetch" "Hcont".
+    iApply fetch_spec; iFrameCapSolve.
+    iNext. iIntros "(HPC & Hfetch & Hr_t1 & Hr_t2 & Hr_t3 & Hpc_b & Ha_entry)".
+    unfocus_block "Hfetch" "Hcont" as "Hprog".
+
+    focus_block 1 "Hprog" as amid1 Hamid1 "Hprog" "Hcont". cbn [length map encodeInstrsW] in * |-.
+    iGo "Hprog". (* PC is now at b_m *)
     (* we are now ready to use the malloc subroutine spec. For this we prepare the registers *)
     iDestruct (big_sepM_insert _ _ r_t3 with "[$Hregs $Hr_t3]") as "Hregs".
       by rewrite lookup_delete_ne // lookup_delete.
@@ -594,14 +301,10 @@ Section macros.
     { rewrite !dom_insert_L dom_delete_L Hrmap_dom.
       rewrite !difference_difference_L !singleton_union_difference_L !all_registers_union_l.
       f_equal. set_solver-. }
-    (* { lia. } *)
     iNext.
-    rewrite updatePcPerm_cap_non_E.
-    2: { eapply isCorrectPC_range_perm_non_E; eauto.
-         generalize (contiguous_between_length _ _ _ Hcont_rest). cbn.
-         clear; solve_addr. }
+    rewrite updatePcPerm_cap_non_E; [| solve_pure].
     iIntros "((Hna & Hregs) & Hr_t0 & HPC & Hbe) /=".
-    iDestruct "Hbe" as (b e size' Hsize' Hbe) "(Hr_t1 & Hbe)". inversion Hsize';subst size'.
+    iDestruct "Hbe" as (b e size' Hsize' Hbe) "(Hr_t1 & Hbe)". inversion Hsize'; subst size'.
     iDestruct (big_sepM_delete _ _ r_t3 with "Hregs") as "[Hr_t3 Hregs]".
       by rewrite lookup_insert_ne // lookup_insert //.
       rewrite delete_insert_ne // delete_insert_delete.
@@ -609,39 +312,78 @@ Section macros.
     iDestruct (big_sepM_delete _ _ r_t5 with "Hregs") as "[Hr_t5 Hregs]".
       by (repeat (rewrite lookup_insert_ne //;[]); rewrite lookup_insert //).
       repeat (rewrite delete_insert_ne //;[]). rewrite delete_insert_delete.
-    (* move r_t0 r_t5 *)
-    iPrologue "Hprog".
-    iApply (wp_move_success_reg with "[$HPC $Hi $Hr_t0 $Hr_t5]");
-      [apply decode_encode_instrW_inv|iCorrectPC link a_last|iContiguous_next Hcont_rest 6|auto|..].
-    iEpilogue "(HPC & Hi & Hr_t0 & Hr_t5)"; iCombine "Hi" "Hprog_done" as "Hprog_done".
-    (* move r_t5 0 *)
-    destruct l';[| by inversion Hlength_rest].
-    iPrologue "Hprog".
-    apply contiguous_between_last with (ai:=a5) in Hcont_rest as Hlast;[|auto].
-    iApply (wp_move_success_z with "[$HPC $Hi $Hr_t5]");
-      [apply decode_encode_instrW_inv|iCorrectPC link a_last|apply Hlast|auto|..].
-    iEpilogue "(HPC & Hi & Hr_t5)"; iCombine "Hi" "Hprog_done" as "Hprog_done".
+    (* back our program, in the continuation of malloc *)
+    iGo "Hprog".
+    unfocus_block "Hprog" "Hcont" as "Hprog".
     (* continuation *)
-    iApply "Hφ".
-    iFrame "HPC". iSplitL "Hprog_done".
-    { rewrite Heqapp. repeat (iDestruct "Hprog_done" as "[$ Hprog_done]"). iFrame. done. }
-    iFrame.
-    iDestruct (big_sepM_insert _ _ r_t5 with "[$Hregs $Hr_t5]") as "Hregs".
-      repeat (rewrite lookup_insert_ne //;[]). apply lookup_delete.
-    iDestruct (big_sepM_insert _ _ r_t3 with "[$Hregs $Hr_t3]") as "Hregs".
-      repeat (rewrite lookup_insert_ne //;[]).
-      rewrite lookup_delete_ne // lookup_delete //.
-    repeat (rewrite (insert_commute _ r_t5) //;[]).
-    rewrite insert_delete -(delete_insert_ne _ _ r_t5) //.
-    rewrite (insert_commute _ r_t5 r_t2) // (delete_insert_ne _ r_t3 r_t2)//.
-    rewrite (insert_commute _ r_t4 r_t2) // insert_insert.
-    rewrite (insert_commute _ r_t3 r_t2) //.
-    rewrite -(delete_insert_ne _ r_t3) // insert_delete.
-    iFrame.
-    iExists b,e. iFrame. auto. iIntros (v) "[Hφ|Hφ] /=". iApply "Hψ". iFrame. iSimplifyEq. iApply "Hψ". iFrame.
+    iApply "Hφ". changePCto (a_first ^+ 18%nat)%a.
+    iFrame. iSplitL "Hr_t1 Hbe".
+    { iExists _,_. iFrame. iPureIntro; eauto. }
+    { iDestruct (big_sepM_insert _ _ r_t5 with "[$Hregs $Hr_t5]") as "Hregs".
+        repeat (rewrite lookup_insert_ne //;[]). apply lookup_delete.
+      iDestruct (big_sepM_insert _ _ r_t3 with "[$Hregs $Hr_t3]") as "Hregs".
+        repeat (rewrite lookup_insert_ne //;[]).
+        rewrite lookup_delete_ne // lookup_delete //.
+      repeat (rewrite (insert_commute _ r_t5) //;[]).
+      rewrite insert_delete -(delete_insert_ne _ _ r_t5) //.
+      rewrite (insert_commute _ r_t5 r_t2) // (delete_insert_ne _ r_t3 r_t2)//.
+      rewrite (insert_commute _ r_t4 r_t2) // insert_insert.
+      rewrite (insert_commute _ r_t3 r_t2) //.
+      rewrite -(delete_insert_ne _ r_t3) // insert_delete. iFrame. }
+    { iIntros (v) "[Hφ|Hφ] /=". iApply "Hψ". iFrame. iSimplifyEq. eauto. }
   Qed.
 
-  
+  (* malloc spec - alternative formulation *)
+  Lemma malloc_spec φ size cont pc_p pc_b pc_e a_first
+        b_link e_link a_link f_m a_entry mallocN b_m e_m EN rmap :
+    ExecPCPerm pc_p →
+    SubBounds pc_b pc_e a_first (a_first ^+ length (malloc_instrs f_m size))%a →
+    withinBounds (RW, b_link, e_link, a_entry) = true →
+    (a_link + f_m)%a = Some a_entry →
+    dom (gset RegName) rmap = all_registers_s ∖ {[ PC; r_t0 ]} →
+    ↑mallocN ⊆ EN →
+    (size > 0)%Z →
+
+    (* malloc program and subroutine *)
+    ▷ codefrag a_first (malloc_instrs f_m size)
+    ∗ na_inv logrel_nais mallocN (malloc_inv b_m e_m)
+    ∗ na_own logrel_nais EN
+    (* we need to assume that the malloc capability is in the linking table at offset f_m *)
+    ∗ ▷ pc_b ↦ₐ inr (RO,b_link,e_link,a_link)
+    ∗ ▷ a_entry ↦ₐ inr (E,b_m,e_m,b_m)
+    (* register state *)
+    ∗ ▷ PC ↦ᵣ inr (pc_p,pc_b,pc_e,a_first)
+    ∗ ▷ r_t0 ↦ᵣ cont
+    ∗ ▷ ([∗ map] r_i↦w_i ∈ rmap, r_i ↦ᵣ w_i)
+    (* continuation *)
+    ∗ ▷ (PC ↦ᵣ inr (pc_p,pc_b,pc_e, (a_first ^+ length (malloc_instrs f_m size))%a)
+         ∗ codefrag a_first (malloc_instrs f_m size)
+         ∗ pc_b ↦ₐ inr (RO,b_link,e_link,a_link)
+         ∗ a_entry ↦ₐ inr (E,b_m,e_m,b_m)
+         (* the newly allocated region *)
+         ∗ (∃ (b e : Addr),
+            ⌜(b + size)%a = Some e⌝
+            ∗ r_t1 ↦ᵣ inr (RWX,b,e,b)
+            ∗ [[b,e]] ↦ₐ [[region_addrs_zeroes b e]])
+         ∗ r_t0 ↦ᵣ cont
+         ∗ na_own logrel_nais EN
+         ∗ ([∗ map] r_i↦w_i ∈ (<[r_t2:=inl 0%Z]>
+                               (<[r_t3:=inl 0%Z]>
+                                (<[r_t4:=inl 0%Z]>
+                                 (<[r_t5:=inl 0%Z]> (delete r_t1 rmap))))), r_i ↦ᵣ w_i)
+         (* the newly allocated region is fresh in the current world *)
+         (* ∗ ⌜Forall (λ a, a ∉ dom (gset Addr) (std W)) (region_addrs b e)⌝ *)
+         -∗ WP Seq (Instr Executable) {{ φ }})
+    ⊢
+      WP Seq (Instr Executable) {{ λ v, φ v ∨ ⌜v = FailedV⌝ }}.
+  Proof.
+    iIntros (Hvpc Hcont Hwb Ha_entry Hrmap_dom HmallocN Hsize)
+            "(>Hprog & #Hmalloc & Hna & >Hpc_b & >Ha_entry & >HPC & >Hr_t0 & >Hregs & Hφ)".
+    iApply malloc_spec_alt; iFrameCapSolve; eauto. iFrame. iFrame "Hmalloc".
+    iSplitL. iNext. eauto. eauto.
+  Qed.
+
+
   (* -------------------------------------- RCLEAR ----------------------------------- *)
   (* the following macro clears registers in r. a denotes the list of addresses
      containing the instructions for the clear: |a| = |r| *)
